desync/lakefile.lean
@@ -1,0 +1,10 @@
+import Lake
+open Lake DSL
+
+package «sqlar-cas-desync» where
+
+require «sqlar-cas-sqlar» from ".." / "sqlar"
+require «sqlar-cas-index» from ".." / "index"
+
+@[default_target]
+lean_lib SqlarCasDesync
